# Problem 200: Determine \(a\) for a Curl-Free Vector Field

## Problem Statement

For what value of the constant \(a\) does the vector field

$$
\mathbf{A} = (a x y - z^3)\mathbf{i} + (a-2)x^2 \mathbf{j} + (1-a)x z^2 \mathbf{k}
$$

have an identically zero curl (\(\nabla \times \mathbf{A} = \mathbf{0}\))?

## Solution

### Step 1: Compute the Curl

Use the determinant form of the curl:

$$
\nabla \times \mathbf{A} =
\begin{vmatrix}
\mathbf{i} & \mathbf{j} & \mathbf{k} \\
\frac{\partial}{\partial x} & \frac{\partial}{\partial y} & \frac{\partial}{\partial z} \\
a x y - z^3 & (a-2)x^2 & (1-a)x z^2
\end{vmatrix}.
$$

Compute each component.

### Step 2: Components of the Curl

- \( \mathbf{i} \)-component:
  $$
  \frac{\partial}{\partial y}[(1-a)x z^2] - \frac{\partial}{\partial z}[(a-2)x^2] = 0 - 0 = 0.
  $$

- \( \mathbf{j} \)-component:
  $$
  -\left( \frac{\partial}{\partial x}[(1-a)x z^2] - \frac{\partial}{\partial z}[a x y - z^3] \right)
  = -\left( (1-a) z^2 - (-3z^2) \right) = -(4 - a) z^2.
  $$

- \( \mathbf{k} \)-component:
  $$
  \frac{\partial}{\partial x}[(a-2)x^2] - \frac{\partial}{\partial y}[a x y - z^3]
  = (2a - 4)x - a x = (a - 4)x.
  $$

### Step 3: Set the Curl to Zero

For the curl to vanish identically for all \(x, z\), both coefficients must be zero:

$$
4 - a = 0, \qquad a - 4 = 0.
$$

Thus, \(a = 4\).

## Answer

$$
\boxed{a = 4}
$$
