# Problem 181: Solenoidal Vector Fields

## Problem Statement

Show that $\mathbf{A} = (2x^2 + 8xy^2z)\mathbf{i} + (3x^3y - 3xy)\mathbf{j} - (4y^2z^2 + 2x^3z)\mathbf{k}$ is not solenoidal, but $\mathbf{B} = xyz^2\mathbf{A}$ is solenoidal.

## Solution

### Part 1: Show that $\mathbf{A}$ is Not Solenoidal

### Step 1: Calculate the Divergence of $\mathbf{A}$

The divergence is:

$$\nabla \cdot \mathbf{A} = \left(\frac{\partial}{\partial x}\mathbf{i} + \frac{\partial}{\partial y}\mathbf{j} + \frac{\partial}{\partial z}\mathbf{k}\right) \cdot \left\{(2x^2 + 8xy^2z)\mathbf{i} + (3x^3y - 3xy)\mathbf{j} - (4y^2z^2 + 2x^3z)\mathbf{k}\right\}$$

Expanding:

$$\nabla \cdot \mathbf{A} = \frac{\partial}{\partial x}(2x^2 + 8xy^2z) + \frac{\partial}{\partial y}(3x^3y - 3xy) - \frac{\partial}{\partial z}(4y^2z^2 + 2x^3z)$$

### Step 2: Evaluate Partial Derivatives

Calculating each term:

- $\frac{\partial}{\partial x}(2x^2 + 8xy^2z) = 4x + 8y^2z$
- $\frac{\partial}{\partial y}(3x^3y - 3xy) = 3x^3 - 3x$
- $\frac{\partial}{\partial z}(4y^2z^2 + 2x^3z) = 8y^2z + 2x^3$

### Step 3: Combine Terms

$$\nabla \cdot \mathbf{A} = (4x + 8y^2z) + (3x^3 - 3x) - (8y^2z + 2x^3)$$

$$= 4x + 8y^2z + 3x^3 - 3x - 8y^2z - 2x^3$$

$$= x + x^3$$

### Step 4: Conclusion for $\mathbf{A}$

Since $\nabla \cdot \mathbf{A} = x + x^3 \neq 0$, the vector field $\mathbf{A}$ is **not solenoidal**.

### Part 2: Show that $\mathbf{B} = xyz^2\mathbf{A}$ is Solenoidal

### Step 5: Expand $\mathbf{B}$

$$\mathbf{B} = xyz^2 \left\{(2x^2 + 8xy^2z)\mathbf{i} + (3x^3y - 3xy)\mathbf{j} - (4y^2z^2 + 2x^3z)\mathbf{k}\right\}$$

Expanding:

$$\mathbf{B} = (2x^3yz^2 + 8x^2y^3z^3)\mathbf{i} + (3x^4y^2z^2 - 3x^2y^2z^2)\mathbf{j} - (4xy^3z^4 + 2x^4yz^3)\mathbf{k}$$

### Step 6: Calculate the Divergence of $\mathbf{B}$

$$\nabla \cdot \mathbf{B} = \frac{\partial}{\partial x}(2x^3yz^2 + 8x^2y^3z^3) + \frac{\partial}{\partial y}(3x^4y^2z^2 - 3x^2y^2z^2) + \frac{\partial}{\partial z}(-4xy^3z^4 - 2x^4yz^3)$$

### Step 7: Evaluate Partial Derivatives

Calculating each term:

- $\frac{\partial}{\partial x}(2x^3yz^2 + 8x^2y^3z^3) = 6x^2yz^2 + 16xy^3z^3$
- $\frac{\partial}{\partial y}(3x^4y^2z^2 - 3x^2y^2z^2) = 6x^4yz^2 - 6x^2yz^2$
- $\frac{\partial}{\partial z}(-4xy^3z^4 - 2x^4yz^3) = -16xy^3z^3 - 6x^4yz^2$

### Step 8: Combine Terms

$$\nabla \cdot \mathbf{B} = (6x^2yz^2 + 16xy^3z^3) + (6x^4yz^2 - 6x^2yz^2) - (16xy^3z^3 + 6x^4yz^2)$$

$$= 6x^2yz^2 + 16xy^3z^3 + 6x^4yz^2 - 6x^2yz^2 - 16xy^3z^3 - 6x^4yz^2$$

$$= 0$$

### Step 9: Conclusion for $\mathbf{B}$

Since $\nabla \cdot \mathbf{B} = 0$, the vector field $\mathbf{B}$ is **solenoidal**.

## Answer

**Part 1:** $\mathbf{A}$ is not solenoidal:

$$\boxed{\nabla \cdot \mathbf{A} = x + x^3 \neq 0}$$

**Part 2:** $\mathbf{B}$ is solenoidal:

$$\boxed{\nabla \cdot \mathbf{B} = 0}$$
